theories/lang_generic.v
@@ -1,42 +1,42 @@
-From gitrees Require Import prelude.
-From Equations Require Import Equations.
-Require Import List.
-Import ListNotations.
+(* From gitrees Require Import prelude. *)
+(* From Equations Require Import Equations. *)
+(* Require Import List. *)
+(* Import ListNotations. *)
 
-(** XXX: We /NEED/ this line for [Equations Derive] to work,
- this flag is globally unset by std++, but Equations need obligations to be transparent. *)
-Set Transparent Obligations.
+(* (** XXX: We /NEED/ this line for [Equations Derive] to work, *)
+(*  this flag is globally unset by std++, but Equations need obligations to be transparent. *) *)
+(* Set Transparent Obligations. *)
 
-Derive NoConfusion NoConfusionHom for list.
+(* Derive NoConfusion NoConfusionHom for list. *)
 
-Definition scope := (list unit).
+(* Definition scope := (list unit). *)
 
-(** Variables in a context *)
-Inductive var : scope → Type :=
-| Vz : forall {S : scope} {s}, var (s::S)
-| Vs : forall {S : scope} {s}, var S -> var (s::S)
-.
-Derive Signature NoConfusion for var.
+(* (** Variables in a context *) *)
+(* Inductive var : scope → Type := *)
+(* | Vz : forall {S : scope} {s}, var (s::S) *)
+(* | Vs : forall {S : scope} {s}, var S -> var (s::S) *)
+(* . *)
+(* Derive Signature NoConfusion for var. *)
 
-Inductive tyctx (ty : Type) : scope → Type :=
-| empC : tyctx ty []
-| consC : forall{Γ}, ty → tyctx ty Γ → tyctx ty (()::Γ)
-.
-Arguments empC {_}.
-Arguments consC {_ _} _ _.
+(* Inductive tyctx (ty : Type) : scope → Type := *)
+(* | empC : tyctx ty [] *)
+(* | consC : forall{Γ}, ty → tyctx ty Γ → tyctx ty (()::Γ) *)
+(* . *)
+(* Arguments empC {_}. *)
+(* Arguments consC {_ _} _ _. *)
 
-Equations list_of_tyctx {S ty} (Γ : tyctx ty S) : list ty :=
-  list_of_tyctx empC := [];
-  list_of_tyctx (consC τ Γ') := τ::list_of_tyctx Γ'.
+(* Equations list_of_tyctx {S ty} (Γ : tyctx ty S) : list ty := *)
+(*   list_of_tyctx empC := []; *)
+(*   list_of_tyctx (consC τ Γ') := τ::list_of_tyctx Γ'. *)
 
-Equations tyctx_app {S1 S2 ty} (c1 : tyctx ty S1) (c2 : tyctx ty S2) : tyctx ty (S1++S2) :=
-  tyctx_app empC         c2 := c2;
-  tyctx_app (consC τ c1) c2 := consC τ (tyctx_app c1 c2).
+(* Equations tyctx_app {S1 S2 ty} (c1 : tyctx ty S1) (c2 : tyctx ty S2) : tyctx ty (S1++S2) := *)
+(*   tyctx_app empC         c2 := c2; *)
+(*   tyctx_app (consC τ c1) c2 := consC τ (tyctx_app c1 c2). *)
 
-Inductive typed_var {ty : Type}: forall {S}, tyctx ty S → var S → ty → Prop :=
-| typed_var_Z S (τ : ty) (Γ : tyctx ty S) :
-  typed_var (consC τ Γ) Vz τ
-| typed_var_S S (τ τ' : ty) (Γ : tyctx ty S) v :
-  typed_var Γ v τ →
-  typed_var (consC τ' Γ) (Vs v) τ
-.
+(* Inductive typed_var {ty : Type}: forall {S}, tyctx ty S → var S → ty → Prop := *)
+(* | typed_var_Z S (τ : ty) (Γ : tyctx ty S) : *)
+(*   typed_var (consC τ Γ) Vz τ *)
+(* | typed_var_S S (τ τ' : ty) (Γ : tyctx ty S) v : *)
+(*   typed_var Γ v τ → *)
+(*   typed_var (consC τ' Γ) (Vs v) τ *)
+(* . *)
